coq/SnakeletWp.v
@@ -1,0 +1,326 @@
+From iris.proofmode Require Import proofmode.
+From iris.program_logic Require Import lifting.
+From iris.base_logic.lib Require Export gen_heap.
+From iris.algebra Require Import dfrac.
+From stdpp Require Import fin_maps fin_map_dom.
+Require Import SnakeletLang.
+Import snakelet_notation.
+
+Local Notation "l ↦{ dq } v" := (pointsto l dq v)
+  (at level 20, dq custom dfrac at level 1, format "l  ↦{ dq }  v") : bi_scope.
+Local Notation "l ↦ v" := (pointsto l (DfracOwn 1) v)
+  (at level 20, format "l  ↦  v") : bi_scope.
+
+Class snakelet_heapGS_gen hlc Σ := SnakeletHeapGS {
+  #[global] snakelet_invGS :: invGS_gen hlc Σ;
+  #[global] snakelet_gen_heapG :: gen_heapGS loc sn_val Σ;
+}.
+Global Existing Instance snakelet_invGS.
+Global Existing Instance snakelet_gen_heapG.
+Notation snakelet_heapGS := (snakelet_heapGS_gen HasLc).
+
+Section snakelet_wp.
+  Context `{!snakelet_heapGS_gen hlc Σ}.
+
+  Definition snakelet_state_interp (σ : sn_state) (ns : nat) (κs : list observation) (nt : nat) : iProp Σ :=
+    gen_heap_interp σ.
+
+  Global Program Instance snakelet_irisGS : irisGS_gen hlc snakelet_lang Σ := {|
+    iris_invGS := snakelet_invGS;
+    state_interp := snakelet_state_interp;
+    fork_post _ := True%I;
+    num_laters_per_step _ := 0%nat;
+    state_interp_mono _ _ _ _ := fupd_intro _ _
+  |}.
+  Global Opaque iris_invGS.
+
+  (** Determinant lemmas — pure steps *)
+  Lemma reducible_pure_step e e' σ :
+    pure_step e e' → reducible e σ.
+  Proof.
+    intros Hpure. eexists [], e', σ, [].
+    eapply (PrimPureStep _ σ). exact Hpure.
+  Qed.
+
+  Lemma reducible_no_obs_pure_step e e' σ :
+    pure_step e e' → reducible_no_obs e σ.
+  Proof.
+    intros Hpure. eexists e', σ, [].
+    eapply (PrimPureStep _ σ). exact Hpure.
+  Qed.
+
+  Lemma prim_binop_det op v1 v2 σ κ e2 σ2 efs :
+    prim_step (BinOp op (Val v1) (Val v2)) σ κ e2 σ2 efs →
+    κ = [] ∧ σ2 = σ ∧ efs = [] ∧ e2 = Val (binop_eval op v1 v2).
+  Proof.
+    intros Hprim. inversion Hprim; [| inversion H].
+    inversion H; subst. auto.
+  Qed.
+
+  Lemma prim_let_det x v e σ κ e2 σ2 efs :
+    prim_step (Let x (Val v) e) σ κ e2 σ2 efs →
+    κ = [] ∧ σ2 = σ ∧ efs = [] ∧ e2 = subst x v e.
+  Proof.
+    intros Hprim. inversion Hprim; [| inversion H].
+    inversion H; subst. auto.
+  Qed.
+
+  Lemma prim_if_true_det e1 e2 σ κ e2' σ2 efs :
+    prim_step (If (Val (LitBool true)) e1 e2) σ κ e2' σ2 efs →
+    κ = [] ∧ σ2 = σ ∧ efs = [] ∧ e2' = e1.
+  Proof.
+    intros Hprim. inversion Hprim; [| inversion H].
+    inversion H; subst. auto.
+  Qed.
+
+  Lemma prim_if_false_det e1 e2 σ κ e2' σ2 efs :
+    prim_step (If (Val (LitBool false)) e1 e2) σ κ e2' σ2 efs →
+    κ = [] ∧ σ2 = σ ∧ efs = [] ∧ e2' = e2.
+  Proof.
+    intros Hprim. inversion Hprim; [| inversion H].
+    inversion H; subst. auto.
+  Qed.
+
+  (** Head-step determinant lemmas *)
+  Lemma head_load_det l σ e2 σ2 efs :
+    head_step (Load (Val (LitLoc l))) σ e2 σ2 efs →
+    ∃ v, σ !! l = Some v ∧ e2 = Val v ∧ σ2 = σ ∧ efs = [].
+  Proof. intros H. inversion H; subst. eauto. Qed.
+
+  Lemma head_store_det l v σ e2 σ2 efs :
+    head_step (Store (Val (LitLoc l)) (Val v)) σ e2 σ2 efs →
+    is_Some (σ !! l) ∧ e2 = Val LitUnit ∧ σ2 = <[l:=v]> σ ∧ efs = [].
+  Proof. intros H. inversion H; subst. split; [done|]. auto. Qed.
+
+  Lemma head_alloc_det v σ e2 σ2 efs :
+    head_step (Alloc (Val v)) σ e2 σ2 efs →
+    ∃ l, σ !! l = None ∧ e2 = Val (LitLoc l) ∧ σ2 = <[l:=v]> σ ∧ efs = [].
+  Proof. intros H. inversion H; subst. eauto. Qed.
+
+  Lemma head_faa_det l v σ e2 σ2 efs :
+    head_step (FAA (Val (LitLoc l)) (Val v)) σ e2 σ2 efs →
+    ∃ z, σ !! l = Some (LitInt z) ∧
+         e2 = Val (LitInt z) ∧ σ2 = <[l:=LitInt (z + lit_as_z v)]> σ ∧ efs = [].
+  Proof. intros H. inversion H; subst. eauto. Qed.
+
+  Lemma head_fork_det e σ e2 σ2 efs :
+    head_step (Fork e) σ e2 σ2 efs →
+    e2 = Val LitUnit ∧ σ2 = σ ∧ efs = [e].
+  Proof. intros H. inversion H; subst. auto. Qed.
+
+  Lemma prim_load_det l σ κ e2 σ2 efs v :
+    σ !! l = Some v →
+    prim_step (Load (Val (LitLoc l))) σ κ e2 σ2 efs →
+    κ = [] ∧ σ2 = σ ∧ efs = [] ∧ e2 = Val v.
+  Proof.
+    intros Hlookup Hprim.
+    inversion Hprim as [e0 σ0 e0' Hpure | e0 σ0 e0' σ0' efs0 Hhead]; subst;
+      [exfalso; inversion Hpure|].
+    edestruct head_load_det as (v'&Hlook'&->&->&->); eauto.
+    assert (v = v') by congruence. subst v'. auto.
+  Qed.
+
+  Lemma prim_store_det l v σ κ e2 σ2 efs :
+    is_Some (σ !! l) →
+    prim_step (Store (Val (LitLoc l)) (Val v)) σ κ e2 σ2 efs →
+    κ = [] ∧ σ2 = <[l:=v]> σ ∧ efs = [] ∧ e2 = Val LitUnit.
+  Proof.
+    intros Hlookup Hprim.
+    inversion Hprim as [e0 σ0 e0' Hpure | e0 σ0 e0' σ0' efs0 Hhead]; subst;
+      [exfalso; inversion Hpure|].
+    edestruct head_store_det as (?&->&->&->); eauto.
+  Qed.
+
+  Lemma prim_alloc_det v σ κ e2 σ2 efs :
+    prim_step (Alloc (Val v)) σ κ e2 σ2 efs →
+    ∃ l, σ !! l = None ∧ κ = [] ∧ σ2 = <[l:=v]> σ ∧ efs = [] ∧ e2 = Val (LitLoc l).
+  Proof.
+    intros Hprim.
+    inversion Hprim as [e0 σ0 e0' Hpure | e0 σ0 e0' σ0' efs0 Hhead]; subst;
+      [exfalso; inversion Hpure|].
+    pose proof (head_alloc_det v σ e2 σ2 efs Hhead) as (l&Hfree&Heq&Heq2&Heq3).
+    rewrite Heq Heq2 Heq3.
+    exists l; split; [exact Hfree|]; auto.
+  Qed.
+
+  (** Pure WP lemmas *)
+  Lemma wp_binop s E op v1 v2 Φ :
+    ▷ Φ (binop_eval op v1 v2) -∗
+    WP BinOp op (Val v1) (Val v2) @ s; E {{ Φ }}.
+  Proof.
+    iIntros "HΦ".
+    iApply wp_lift_pure_step_no_fork; [ | | ].
+    - intros σ. destruct s.
+      + pose proof (reducible_no_obs_pure_step
+            (BinOp op (Val v1) (Val v2)) (Val (binop_eval op v1 v2)) σ
+            (PureBinOp op v1 v2)) as Hred.
+        apply reducible_no_obs_reducible, Hred.
+      + simpl. reflexivity.
+    - intros κ σ1 e2 σ2 efs Hprim.
+      pose proof (prim_binop_det _ _ _ _ _ _ _ _ Hprim) as (->&->&->&_); done.
+    - iModIntro. iNext. iModIntro. iIntros (κ e2 efs σ Hprim) "Hcred".
+      pose proof (prim_binop_det _ _ _ _ _ _ _ _ Hprim) as [Hκ [Hσ [Hefs He2]]].
+      rewrite He2.
+      iDestruct (lc_weaken 1 with "Hcred") as "Hcred"; first done.
+      iApply (wp_value' with "HΦ").
+  Qed.
+
+  Lemma wp_let s E x v e2 Φ :
+    ▷ WP subst x v e2 @ s; E {{ Φ }} -∗
+    WP Let x (Val v) e2 @ s; E {{ Φ }}.
+  Proof.
+    iIntros "HΦ".
+    iApply wp_lift_pure_step_no_fork; [ | | ].
+    - intros σ. destruct s.
+      + pose proof (reducible_no_obs_pure_step
+            (Let x (Val v) e2) (subst x v e2) σ
+            (PureLet v x e2)) as Hred.
+        apply reducible_no_obs_reducible, Hred.
+      + simpl. reflexivity.
+    - intros κ σ1 e2' σ2 efs Hprim.
+      pose proof (prim_let_det _ _ _ _ _ _ _ _ Hprim) as (->&->&->&_); done.
+    - iModIntro. iNext. iModIntro. iIntros (κ e2' efs σ Hprim) "Hcred".
+      pose proof (prim_let_det _ _ _ _ _ _ _ _ Hprim) as [Hκ [Hσ [Hefs He2]]].
+      rewrite He2.
+      iDestruct (lc_weaken 1 with "Hcred") as "Hcred"; first done.
+      iFrame "HΦ".
+  Qed.
+
+  Lemma wp_if_true s E e1 e2 Φ :
+    ▷ WP e1 @ s; E {{ Φ }} -∗
+    WP If (Val (LitBool true)) e1 e2 @ s; E {{ Φ }}.
+  Proof.
+    iIntros "HΦ".
+    iApply wp_lift_pure_step_no_fork; [ | | ].
+    - intros σ. destruct s.
+      + pose proof (reducible_no_obs_pure_step
+            (If (Val (LitBool true)) e1 e2) e1 σ
+            (PureIfTrue e1 e2)) as Hred.
+        apply reducible_no_obs_reducible, Hred.
+      + simpl. reflexivity.
+    - intros κ σ1 e2' σ2 efs Hprim.
+      pose proof (prim_if_true_det _ _ _ _ _ _ _ Hprim) as (->&->&->&_); done.
+    - iModIntro. iNext. iModIntro. iIntros (κ e2' efs σ Hprim) "Hcred".
+      pose proof (prim_if_true_det _ _ _ _ _ _ _ Hprim) as [Hκ [Hσ [Hefs He2]]].
+      rewrite He2.
+      iDestruct (lc_weaken 1 with "Hcred") as "Hcred"; first done.
+      iFrame "HΦ".
+  Qed.
+
+  Lemma wp_if_false s E e1 e2 Φ :
+    ▷ WP e2 @ s; E {{ Φ }} -∗
+    WP If (Val (LitBool false)) e1 e2 @ s; E {{ Φ }}.
+  Proof.
+    iIntros "HΦ".
+    iApply wp_lift_pure_step_no_fork; [ | | ].
+    - intros σ. destruct s.
+      + pose proof (reducible_no_obs_pure_step
+            (If (Val (LitBool false)) e1 e2) e2 σ
+            (PureIfFalse e1 e2)) as Hred.
+        apply reducible_no_obs_reducible, Hred.
+      + simpl. reflexivity.
+    - intros κ σ1 e2' σ2 efs Hprim.
+      pose proof (prim_if_false_det _ _ _ _ _ _ _ Hprim) as (->&->&->&_); done.
+    - iModIntro. iNext. iModIntro. iIntros (κ e2' efs σ Hprim) "Hcred".
+      pose proof (prim_if_false_det _ _ _ _ _ _ _ Hprim) as [Hκ [Hσ [Hefs He2]]].
+      rewrite He2.
+      iDestruct (lc_weaken 1 with "Hcred") as "Hcred"; first done.
+      iFrame "HΦ".
+  Qed.
+
+  (** Stateful WP lemmas.
+
+      Puzzle: after [wp_lift_atomic_step], the postcondition is
+      [from_option Φ False (to_val e2)].  We use [wp_lift_step] (which returns
+      [WP e2 {{ Φ }}]) and handle the pure step directly — this avoids the
+      [from_option] wrinkle entirely. *)
+
+  Lemma wp_load s E l v Φ :
+    l ↦ v -∗
+    (l ↦ v -∗ Φ v) -∗
+    WP (! (LitLoc l))%S @ s; E {{ Φ }}.
+  Proof.
+    iIntros "Hl HΦ". iApply wp_lift_step; [done|].
+    iIntros (σ1 ns κ κs nt) "Hσ".
+    iDestruct (gen_heap_valid with "Hσ Hl") as %Hlookup.
+    iApply fupd_mask_intro; [set_solver|]. iIntros "Hclose". iSplit.
+    { iPureIntro. destruct s; [|done]. apply reducible_no_obs_reducible.
+      eexists _, _, []. eapply (PrimHeadStep (Load _) σ1).
+      eapply (HeadLoad l v σ1). done. }
+    iNext. iIntros (e2 σ2 efs Hprim) "Hcred".
+    iDestruct (lc_weaken 1 with "Hcred") as "Hcred"; first done.
+    pose proof (prim_load_det l σ1 κ e2 σ2 efs v Hlookup Hprim) as [Hκ [Hσ2 [Hefs He2]]].
+    rewrite He2 Hκ Hσ2 Hefs.
+    iMod "Hclose". iModIntro. iFrame "Hσ".
+    iSpecialize ("HΦ" with "Hl").
+    iSplitL.
+    { rewrite wp_unfold /wp_pre /=. iModIntro. iExact "HΦ". }
+    { done. }
+  Qed.
+
+  Lemma wp_store s E l v (w : sn_val) Φ :
+    l ↦ v -∗
+    (l ↦ w -∗ Φ LitUnit) -∗
+    WP (LitLoc l <- w)%S @ s; E {{ Φ }}.
+  Proof.
+    iIntros "Hl HΦ". iApply wp_lift_step; [done|].
+    iIntros (σ1 ns κ κs nt) "Hσ".
+    iDestruct (gen_heap_valid with "Hσ Hl") as %Hlookup.
+    iApply fupd_mask_intro; [set_solver|]. iIntros "Hclose". iSplit.
+    { iPureIntro. destruct s; [|done]. apply reducible_no_obs_reducible.
+      eexists _, _, []. eapply (PrimHeadStep (Store _ _) σ1).
+      eapply (HeadStore l w σ1). eauto. }
+    iNext. iIntros (e2 σ2 efs Hprim) "Hcred".
+    iDestruct (lc_weaken 1 with "Hcred") as "Hcred"; first done.
+    assert (is_Some (σ1 !! l)). { eexists; eauto. }
+    pose proof (prim_store_det l w σ1 κ e2 σ2 efs H Hprim) as [Hκ [Hσ2 [Hefs He2]]].
+    rewrite He2 Hκ Hσ2 Hefs.
+    iMod (gen_heap_update with "Hσ Hl") as "[Hσ Hl]".
+    iMod "Hclose". iModIntro. iFrame "Hσ".
+    iSpecialize ("HΦ" with "Hl").
+    iSplitL.
+    { rewrite wp_unfold /wp_pre /=. iModIntro. iExact "HΦ". }
+    { done. }
+  Qed.
+
+  Lemma fresh_loc (σ : sn_state) : ∃ l, σ !! l = None.
+  Proof.
+    set (d := @dom (gmap loc sn_val) (gset loc) (@gset_dom loc _ _ sn_val) σ).
+    destruct (exist_fresh d) as [l Hl].
+    exists l. eapply (not_elem_of_dom_1 (M:=gmap loc) (D:=gset loc)). exact Hl.
+  Qed.
+
+  Lemma wp_alloc s E v Φ :
+    (∀ l, l ↦ v -∗ Φ (LitLoc l)) -∗
+    WP Alloc (Val v) @ s; E {{ Φ }}.
+  Proof.
+    iIntros "HΦ". iApply wp_lift_step; [done|].
+    iIntros (σ1 ns κ κs nt) "Hσ".
+    edestruct fresh_loc as [l Hfree].
+    iApply fupd_mask_intro; [set_solver|]. iIntros "Hclose". iSplit.
+    { iPureIntro. destruct s; [|done]. apply reducible_no_obs_reducible.
+      eexists (Val (LitLoc l)), (<[l:=v]> σ1), [].
+      eapply (PrimHeadStep (Alloc _) σ1).
+      eapply (HeadAlloc v σ1 l). done. }
+    iNext. iIntros (e2 σ2 efs Hprim) "Hcred".
+    iDestruct (lc_weaken 1 with "Hcred") as "Hcred"; first done.
+    pose proof (prim_alloc_det v σ1 κ e2 σ2 efs Hprim) as (l'&Hfree2&Hκ&Hσ2&Hefs&He2).
+    rewrite He2 Hκ Hσ2 Hefs.
+    iMod (gen_heap_alloc with "Hσ") as "[Hσ Hl]"; first done.
+    iDestruct "Hl" as "[Hl _]".
+    iMod "Hclose". iModIntro. iFrame "Hσ".
+    iSpecialize ("HΦ" $! l' with "Hl").
+    iSplitL.
+    { rewrite wp_unfold /wp_pre /=. iModIntro. iExact "HΦ". }
+    { done. }
+  Qed.
+
+End snakelet_wp.
+
+(** Automation: repeatedly apply pure WP reductions. *)
+Ltac snakelet_pures :=
+  repeat (iApply wp_binop || iApply wp_let || iApply wp_if_true || iApply wp_if_false).
+
+(** Register [IntoVal] so [wp_value] resolves correctly. *)
+Global Instance into_val_val v : IntoVal (Val v) v.
+Proof. done. Qed.
